add scanWithPostCondition

Batteries/Data/Iterators/Scan.lean
@@ -5,256 +5,288 @@ Authors: Chad Sharp
 -/
 
 module
+import Batteries.Data.Bool
 
 public section
-
 namespace Std.Iterators.Types
-
 
 /--
   Internal state for the ScanM combinator
 -/
 structure ScanM (α : Type w) (m : Type w → Type w') (n : Type w → Type w'')
-    (β : Type w) (γ : Type w) (f : γ → β → n γ) where
+    (β : Type w) (γ : Type w) (lift : ⦃α : Type w⦄ → m α → n α)
+    (f : γ → β → PostconditionT n γ)  where
   /-- Inner iterator -/
-  inner : α
+  inner : IterM (α := α) m β
   /-- Current accumulated value -/
   acc : γ
-  /-- Whether we have emitted the initial value
-    (and therefore should begin yielding from the iterator) -/
-  emittedInit : Bool
+  /-- Whether we need to emit the initial value
+    (and therefore have not yet begun yielding from the iterator) -/
+  needsInit : Bool
+
+/-- Internal implementation of the `scanM` combinator. See `IterM.scanM` for the public API. -/
+@[expose]
+public def IterM.InternalCombinators.scanM (lift : ⦃α : Type w⦄ → m α → n α )
+    (f : γ → β → PostconditionT n γ) (acc : γ) (needsInit : Bool) (it : IterM (α := α) m β) :
+    IterM (α := ScanM α m n β γ lift f) n γ :=
+  .mk ⟨it, acc, needsInit⟩ n γ
 
 namespace ScanM
-
 variable {α β γ : Type w} {m : Type w → Type w'} {n : Type w → Type w''}
-  {f : γ → β → n γ} [Iterator α m β]
+  {f : γ → β → PostconditionT n γ} {lift : ⦃α : Type w⦄ → m α → n α} [Iterator α m β]
+
 /--
 `it.IsPlausibleStep` is the proposition that `step` is a possible next step from the `scanM`
 iterator `it`. This is mostly an internal implementation detail used to prove termination.
 -/
-inductive IsPlausibleStep (it : @IterM (ScanM α m n β γ f) n γ) :
-    IterStep (@IterM (ScanM α m n β γ f) n γ) γ → Prop where
-
-  /-- If we haven't emitted anything yet (emittedInit is false),
-      we set it to true and do not update the internal iterator state
+inductive IsPlausibleStep (it : @IterM (ScanM α m n β γ lift f) n γ) :
+    IterStep (@IterM (ScanM α m n β γ lift f) n γ) γ → Prop where
+  /-- If we haven't emitted anything yet (needsInit is true),
+      we set it to false and do not update the internal iterator state
   -/
-  | yieldInit {it' : IterM n γ} {out : γ} :
-      it.internalState.emittedInit = false →
-      it'.internalState.emittedInit = true →
-      it'.internalState.inner = it.internalState.inner →
-      IsPlausibleStep it (.yield it' out)
-  /-- After `emittedInit` is set to true, we yield when the inner iterator does.
-      The resulting state has emittedInit set to true and the updated internal iterator state.
+  | yieldInit :
+      it.internalState.needsInit = true →
+      IsPlausibleStep it (.yield
+        (IterM.InternalCombinators.scanM
+         lift f it.internalState.acc false it.internalState.inner)
+         it.internalState.acc)
+  /-- After `needsInit` is set to false, we yield when the inner iterator does.
+      The resulting state has needsInit set to false and the updated internal iterator state.
   -/
-  | yieldNext {innerIt' : IterM m β} {b : β} {it': IterM n γ} {out : γ}:
-      it.internalState.emittedInit = true
-      → Iterator.IsPlausibleStep ⟨it.internalState.inner⟩ (.yield innerIt' b)
-      → it'.internalState.inner = innerIt'.internalState
-      → it'.internalState.emittedInit = true
-      → IsPlausibleStep it (.yield it' out)
-  /-- After `emittedInit` is set to true, we skip when the inner iterator does.
+  | yieldNext : ∀ {it' b out},
+      it.internalState.needsInit = false →
+      it.internalState.inner.IsPlausibleStep (.yield it' b) →
+      (f it.internalState.acc b).Property out →
+      IsPlausibleStep it (.yield (IterM.InternalCombinators.scanM lift f out false it') out)
+  /-- After `needsInit` is set to false, we skip when the inner iterator does.
       Our resulting state is identical, except with an updated inner iterator
   -/
-  | skip {innerIt' : IterM m β} {it' : IterM n γ}:
-      it.internalState.emittedInit = true
-      → Iterator.IsPlausibleStep ⟨it.internalState.inner⟩ (.skip innerIt')
-      → it' = ⟨{it.internalState with inner := innerIt'.internalState}⟩
-      → IsPlausibleStep it (.skip it')
-  /-- We are done when emittedInit is true and the internal iterator is done -/
+  | skip : ∀ {it'},
+      it.internalState.needsInit = false →
+      it.internalState.inner.IsPlausibleStep (.skip it') →
+      IsPlausibleStep it
+      (.skip (IterM.InternalCombinators.scanM lift f it.internalState.acc false it'))
+  /-- We are done when needsInit is false and the internal iterator is done -/
   | done :
-      it.internalState.emittedInit = true →
-      Iterator.IsPlausibleStep (⟨it.internalState.inner⟩ : IterM m β) .done →
+      it.internalState.needsInit = false →
+      it.internalState.inner.IsPlausibleStep .done →
       IsPlausibleStep it .done
 
-instance instIterator [Monad n] [MonadLiftT m n] :
-    Iterator (ScanM α m n β γ f) n γ where
-
-  IsPlausibleStep := IsPlausibleStep
-  step it := do
-    if h : it.internalState.emittedInit = false then
-      pure <| .deflate <| .yield
-        ⟨{ it.internalState with emittedInit := true }⟩
-        it.internalState.acc
-        (.yieldInit (by simpa using h) rfl rfl)
-    else
-      let innerIt := ⟨it.internalState.inner⟩
-      match hs : (← liftM (Iterator.step innerIt)).inflate with
-      | ⟨.yield inner' a, hp⟩ =>
-        let newAcc ← f it.internalState.acc a
+instance instIterator {α β γ : Type w} {m : Type w → Type w'}
+    {n : Type w → Type w''} {lift : ⦃α : Type w⦄ → m α → n α} {f : γ → β → PostconditionT n γ}
+    [Iterator α m β] [Monad n] :
+    Iterator (ScanM α m n β γ lift f) n γ where
+  IsPlausibleStep := ScanM.IsPlausibleStep
+  step it :=
+    letI : MonadLift m n := ⟨lift (α := _)⟩
+    do
+      if h : it.internalState.needsInit = true then
         pure <| .deflate <| .yield
-          ⟨{it.internalState with inner := inner'.internalState, acc := newAcc}⟩
-          newAcc
-          (.yieldNext (by simpa using h) hp rfl (by simpa using h))
-      | ⟨.skip inner', hp⟩ =>
-        pure <| .deflate <| .skip
-          ⟨{ it.internalState with inner := inner'.internalState }⟩
-          (.skip (by simpa using h) hp rfl)
-      | ⟨.done, hp⟩ =>
-        pure <| .deflate <| .done (.done (by simpa using h) hp)
+          (IterM.InternalCombinators.scanM lift f it.internalState.acc false it.internalState.inner)
+          it.internalState.acc
+          (by exact .yieldInit h)
+      else
+        match (← it.internalState.inner.step).inflate with
+        | .yield inner' b hp => do
+          let ⟨newAcc, h_acc⟩ ← (f it.internalState.acc b).operation
+          pure <| .deflate <| .yield
+            (IterM.InternalCombinators.scanM lift f newAcc false inner')
+            newAcc
+            (by exact .yieldNext (by simpa using h) hp h_acc)
+        | .skip inner' hp =>
+          pure <| .deflate <| .skip
+            (IterM.InternalCombinators.scanM lift f it.internalState.acc false inner')
+            (by exact .skip (by simpa using h) hp)
+        | .done hp =>
+          pure <| .deflate <| .done (by exact .done (by simpa using h) hp)
 
-instance [Monad n] [MonadLiftT m n] :
-    IteratorLoop (ScanM α m n β γ f) n n :=
-  .defaultImplementation
 
-/-- Finiteness relation for `ScanM`-/
-private def finRel (scanIt' scanIt : @IterM (ScanM α m n β γ f) n γ) : Prop :=
-  match scanIt.internalState.emittedInit, scanIt'.internalState.emittedInit with
-  | false, true => True
-  | true, true => (⟨scanIt'.internalState.inner⟩ : IterM m β).IsPlausibleSuccessorOf
-      ⟨scanIt.internalState.inner⟩
-  | _, _ => False
+namespace Finite
+private def Rel [Monad n] [Finite α m] :
+    IterM (α := ScanM α m n β γ lift f) n γ → IterM (α := ScanM α m n β γ lift f) n γ → Prop :=
+  InvImage
+    (Prod.Lex
+      (· < ·)
+      IterM.IsPlausibleSuccessorOf)
+    (fun it => (it.internalState.needsInit, it.internalState.inner))
 
-private theorem acc_finRel_emittedTrue [Finite α m (β := β)]
-    (scanIt : @IterM (ScanM α m n β γ f) n γ)
-    (hemit : scanIt.internalState.emittedInit = true) :
-    Acc finRel scanIt := by
-  generalize hgen : (⟨scanIt.internalState.inner⟩ : IterM m β) = innerIt
-  induction Finite.wf.apply innerIt generalizing scanIt
-  rename_i ih
-  constructor
-  intro scanIt' _
-  by_cases scanIt'.internalState.emittedInit <;> simp_all only [finRel]
-  exact ih ⟨scanIt'.internalState.inner⟩ ‹_› scanIt' ‹_› rfl
+private theorem rel_of_needsInit [Monad n] [Finite α m]
+    {it it' : IterM (α := ScanM α m n β γ lift f) n γ}
+    (h : it'.internalState.needsInit < it.internalState.needsInit) :
+    Rel it' it :=
+  Prod.Lex.left _ _ h
 
-private theorem acc_finRel_emittedFalse [Finite α m (β := β)]
-    (scanIt : @IterM (ScanM α m n β γ f) n γ)
-    (hemit : scanIt.internalState.emittedInit = false) :
-    Acc finRel scanIt := by
-  constructor
-  intro iter' _
-  by_cases iter'.internalState.emittedInit
-  . exact acc_finRel_emittedTrue _ ‹_›
-  -- this leads to a contradiction
-  . simp_all [finRel]
+private theorem rel_of_inner [Monad n] [Finite α m]
+    {it it' : IterM (α := ScanM α m n β γ lift f) n γ}
+    (h : it'.internalState.needsInit = it.internalState.needsInit)
+    (h' : it'.internalState.inner.IsPlausibleSuccessorOf it.internalState.inner) :
+    Rel it' it := by
+  simp only [Rel, InvImage, h]
+  exact Prod.Lex.right _ h'
 
-private theorem acc_finRel [Finite α m (β := β)] (scanIt : @IterM (ScanM α m n β γ f) n γ) :
-    Acc finRel scanIt :=
-  if h : scanIt.internalState.emittedInit
-    then acc_finRel_emittedTrue _ ‹_›
-    else acc_finRel_emittedFalse _ (by simp only [h])
-
-private def instFinRel [Monad m] [Monad n] [MonadLiftT m n] [Finite α m (β := β)] :
-    FinitenessRelation (ScanM α m n β γ f) n where
-  Rel := finRel
-  wf := ⟨acc_finRel⟩
-  subrelation := by
-    rintro _ _ ⟨_, hsucc_eq, hplaus⟩
-    cases hplaus
-      <;> simp_all only [IterStep.successor, Option.some.injEq, reduceCtorEq]
-      <;> subst hsucc_eq
-      <;> simp_all only [finRel]
+private def instFinitenessRelation {α β γ : Type w} {m : Type w → Type w'}
+    {n : Type w → Type w''} [Monad n] [Iterator α m β] {lift : ⦃α : Type w⦄ → m α → n α}
+    {f : γ → β → PostconditionT n γ} [Finite α m] :
+    FinitenessRelation (ScanM α m n β γ lift f) n where
+  Rel := InvImage
+    (Prod.Lex
+      (· < ·)
+      IterM.IsPlausibleSuccessorOf)
+    (fun it => (it.internalState.needsInit, it.internalState.inner))
+  wf := by
+    apply InvImage.wf
+    refine ⟨fun (a, b) => Prod.lexAccessible (WellFounded.apply ?_ a) (WellFounded.apply ?_) b⟩
+    · exact Bool.lt_wfRel.wf
+    · exact Finite.wf
+  subrelation {it it'} h := by
+    obtain ⟨step, hstep, hplaus⟩ := h
+    cases hplaus <;> cases hstep
+    case yieldInit => apply Prod.Lex.left _ _ ‹_›
+    all_goals
+      apply rel_of_inner <;> simp_all only [IterM.InternalCombinators.scanM, IterM.mk]
     . exact IterM.isPlausibleSuccessorOf_of_yield ‹_›
-    . exact IterM.isPlausibleSuccessorOf_of_skip  ‹_›
+    . exact IterM.isPlausibleSuccessorOf_of_skip ‹_›
+end Finite
 
-instance [Finite α m (β := β)] [Monad m] [Monad n] [MonadLiftT m n] :
-    Finite (ScanM α m n β γ f) n :=
-  .of_finitenessRelation instFinRel
+instance instFinite [Finite α m (β := β)] [Monad n] :
+    Finite (ScanM α m n β γ lift f) n :=
+  .of_finitenessRelation Finite.instFinitenessRelation
 
-/-- Productiveness relation for ScanM -/
-private def prodRel (scanIt' scanIt : @IterM (ScanM α m n β γ f) n γ) : Prop :=
-  (⟨scanIt'.internalState.inner⟩ : IterM m β).IsPlausibleSkipSuccessorOf
-    ⟨scanIt.internalState.inner⟩
+private def instProductivenessRelation [Monad n] [Productive α m] :
+    ProductivenessRelation (ScanM α m n β γ lift f) n where
+  Rel := InvImage IterM.IsPlausibleSkipSuccessorOf (ScanM.inner ∘ IterM.internalState)
+  wf := InvImage.wf _ Productive.wf
+  subrelation {it it'} h := by cases h; assumption
 
-private theorem acc_prodRel [Productive α m (β := β)]
-    (scanIt : @IterM (ScanM α m n β γ f) n γ) :
-    Acc prodRel scanIt := by
-  generalize hgen : (⟨scanIt.internalState.inner⟩ : IterM m β) = innerIt
-  induction Productive.wf.apply innerIt generalizing scanIt with grind only [prodRel, Acc]
-
-private def instProdRel [Monad m] [Monad n] [MonadLiftT m n] [Productive α m (β := β)] :
-    ProductivenessRelation (ScanM α m n β γ f) n where
-  Rel := prodRel
-  wf := ⟨acc_prodRel⟩
-  subrelation := by
-    intro _ _ hsucc
-    cases hsucc <;> simp_all [prodRel, IterM.IsPlausibleSkipSuccessorOf]
-
-instance [Productive α m (β := β)] [Monad m] [Monad n] [MonadLiftT m n] :
-    Productive (ScanM α m n β γ f) n :=
-  .of_productivenessRelation instProdRel
+instance instProductive [Monad n] [Productive α m] :
+    Productive (ScanM α m n β γ lift f) n :=
+  Productive.of_productivenessRelation instProductivenessRelation
 
 end ScanM
 end Std.Iterators.Types
 
 namespace Std
-open Std.Iterators.Types
-
-section Combinators
-variable {α β γ : Type w}
-
-section Monadic
-variable {m : Type w → Type w'}
+open Std.Iterators.Types Std.Iterators
 
 /--
-If `it` is an iterator, then `it.scanM f init` is another iterator that folds a
-monadic function `f` over the values emitted by `it`, producing an iterator of
-partial results. The first value emitted by the resulting iterator is always
-`pure init`.
+*Note: This is a very general combinator that requires an advanced understanding of monads,
+dependent types and termination proofs. The variant `scanM` is easier to use and sufficient
+for most use cases.*
 
-The base iterator `it` being monadic in `m`, `f` can return values in any monad `n`
-for which a `MonadLiftT m n` instance is available.
+If `it` is an iterator, then `it.scanWithPostcondition f acc` is another iterator that applies a
+monadic function `f` to accumulate values emitted by `it`. It first emits the initial accumulator
+`acc`, then for each value `b` emitted by `it`, it computes `f acc b` and emits the result.
+
+`f` is expected to return `PostconditionT n γ`. The base iterator `it` being monadic in
+`m`, `n` can be different from `m`, but `it.scanWithPostcondition f acc` expects a `MonadLiftT m n`
+instance. The `PostconditionT` transformer allows the caller to intrinsically prove properties about
+`f`'s return value in the monad `n`, enabling termination proofs depending on the specific behavior
+of `f`.
+
+**Marble diagram (without monadic effects):**
+
+```text
+it                          ---a ---b ---c ---⊥
+it.scanWithPostcondition    -i -a'-ab'-abc'---⊥
+```
+
+(given that `f i a = pure a'`, `f a' b = pure ab'`, `f ab' c = pure abc'`)
+
+**Termination properties:**
+
+* `Finite` instance: only if `it` is finite
+* `Productive` instance: only if `it` is productive
+
+**Performance:**
+
+For each value emitted by the base iterator `it`, this combinator calls `f`.
+-/
+@[inline, expose]
+def IterM.scanWithPostcondition {α β γ : Type w} {m : Type w → Type w'} {n : Type w → Type w''}
+    [MonadLiftT m n] (f : γ → β → PostconditionT n γ) (acc : γ)
+    (it : IterM (α := α) m β) :=
+  IterM.InternalCombinators.scanM (n := n) (fun ⦃_⦄ => monadLift) f acc true it
+
+/--
+If `it` is an iterator, then `it.scanM f acc` is another iterator that applies a monadic
+function `f` to accumulate values emitted by `it`. It first emits the initial accumulator
+`acc`, then for each value `b` emitted by `it`, it computes `f acc b` and emits the result.
+
+The base iterator `it` being monadic in `m`, `f` can return values in any monad `n` for which a
+`MonadLiftT m n` instance is available.
 
 If `f` is pure, then the simpler variant `it.scan` can be used instead.
 
-**Marble diagram (without monadic effects)**
+**Marble diagram (without monadic effects):**
 
 ```text
-it         -------a--b--c--⊥
-it.scanM   init---a'-b'-c'-⊥
+it           ---a ---b ---c ---⊥
+it.scanM     -i -a'-ab'-abc'---⊥
 ```
-(given that `a' ← f init a`, `b' ← f a' b`, `c' ← f b' c`)
+
+(given that `f i a = pure a'`, `f a' b = pure ab'`, `f ab' c = pure abc'`)
 
 **Termination properties:**
-* `Finite` instance: only if `it` is finite.
-* `Productive` instance: only if `it` is productive.
 
-** Performance:**
+* `Finite` instance: only if `it` is finite
+* `Productive` instance: only if `it` is productive
+
+**Performance:**
 
 For each value emitted by the base iterator `it`, this combinator calls `f`.
 -/
 @[inline, expose]
-def IterM.scanM {n : Type w → Type w''} (f : γ → β → n γ) (init : γ) (it : IterM (α := α) m β) :=
-  IterM.mk (ScanM.mk (f := f) (m := m) it.internalState init false) n γ
+def IterM.scanM {α β γ : Type w} {m : Type w → Type w'} {n : Type w → Type w''}
+    [MonadAttach n] [MonadLiftT m n]
+    (f : γ → β → n γ) (acc : γ) (it : IterM (α := α) m β) :=
+  it.scanWithPostcondition (fun a b => PostconditionT.attachLift (f a b)) acc
 
 /--
-If `it` is an iterator, then `it.scan f init` is another iterator that folds a
-pure function `f` over the values emitted by `it`, producing an iterator of
-partial results. The first value emitted by the resulting iterator is always
-`init`.
+If `it` is an iterator, then `it.scan f acc` is another iterator that applies a
+function `f` to accumulate values emitted by `it`. It first emits the initial accumulator
+`acc`, then for each value `b` emitted by `it`, it computes `f acc b` and emits the result.
 
-If `f` is monadic, `it.scanM` can be used instead.
+In situations where `f` is monadic, use `scanM` instead.
 
-**Marble diagram**
+**Marble diagram:**
 
 ```text
-it        -------a--b--c--⊥
-it.scan   init---a'-b'-c'-⊥
+it         ---a ---b ---c ---⊥
+it.scan    -i -a'-ab'-abc'---⊥
 ```
-(given that `a' = f init a`, `b' = f a' b`, `c' = f b' c`)
+
+(given that `f i a = a'`, `f a' b = ab'`, `f ab' c = abc'`)
 
 **Termination properties:**
-* `Finite` instance: only if `it` is finite.
-* `Productive` instance: only if `it` is productive.
 
-** Performance:**
+* `Finite` instance: only if `it` is finite
+* `Productive` instance: only if `it` is productive
+
+**Performance:**
 
 For each value emitted by the base iterator `it`, this combinator calls `f`.
 -/
-
 @[inline, expose]
-def IterM.scan [Monad m]
-    (f : γ → β → γ) (init : γ) (it : IterM (α := α) m β) :=
-  IterM.scanM (m := m) (n := m) (pure <| f · ·) init it
+def IterM.scan {α β γ : Type w} {m : Type w → Type w'}
+    [Monad m] (f : γ → β → γ) (acc : γ) (it : IterM (α := α) m β) :=
+  (it.scanWithPostcondition (fun a b => pure (f a b)) acc : IterM m γ)
 
-end Monadic
 
 @[inline, expose, inherit_doc IterM.scanM]
-def Iter.scanM {n : Type w → Type w''} (f : γ → β → n γ) (init : γ) (it : Iter (α := α) β) :=
-  IterM.scanM f init it.toIterM
+def Iter.scanWithPostcondition {α β γ : Type w} {m : Type w → Type w'}
+    [Monad m] (f : γ → β → PostconditionT m γ) (acc : γ)
+    (it : Iter (α := α) β) :=
+  (letI : MonadLift Id m := ⟨pure⟩; it.toIterM.scanWithPostcondition f acc : IterM m γ)
+
+@[inline, expose, inherit_doc IterM.scanM]
+def Iter.scanM {α β γ : Type w} {n : Type w → Type w''}
+    [Monad n] [MonadAttach n]
+    (f : γ → β → n γ) (acc : γ) (it : Iter (α := α) β) :=
+  letI : MonadLift Id n := ⟨pure⟩
+  it.toIterM.scanM f acc
 
 @[inline, expose, inherit_doc IterM.scan]
-def Iter.scan (f : γ → β → γ) (init : γ) (it : Iter (α := α) β) :=
-  Iter.scanM (n := Id) (pure <| f · ·) init it |>.toIter
-
-end Combinators
+def Iter.scan {α β γ : Type w}
+    (f : γ → β → γ) (acc : γ) (it : Iter (α := α) β) :=
+  it.toIterM.scan f acc |>.toIter
 end Std
